CMRA structure on lists.
Initial commit by Amin Timany.

algebra/list.v
@@ -110,3 +110,273 @@ Instance listCF_contractive F :
 Proof.
   by intros ? A1 A2 B1 B2 n f g Hfg; apply listC_map_ne, cFunctor_contractive.
 Qed.
+
+(* CMRA *)
+Section cmra.
+  Context {A : cmraT}.
+  Implicit Types l : list A.
+  Local Arguments op _ _ !_ !_ / : simpl nomatch.
+
+  Instance list_op : Op (list A) :=
+    fix go l1 l2 := let _ : Op _ := @go in
+    match l1, l2 with
+    | [], _ => l2
+    | _, [] => l1
+    | x :: l1, y :: l2 => x ⋅ y :: l1 ⋅ l2
+    end.
+  Instance list_core : Core (list A) := fmap core.
+
+  Instance list_valid : Valid (list A) := Forall (λ x, ✓ x).
+  Instance list_validN : ValidN (list A) := λ n, Forall (λ x, ✓{n} x).
+
+  Lemma list_lookup_valid l : ✓ l ↔ ∀ i, ✓ (l !! i).
+  Proof.
+    rewrite {1}/valid /list_valid Forall_lookup; split.
+    - intros Hl i. by destruct (l !! i) as [x|] eqn:?; [apply (Hl i)|].
+    - intros Hl i x Hi. move: (Hl i); by rewrite Hi.
+  Qed.
+  Lemma list_lookup_validN n l : ✓{n} l ↔ ∀ i, ✓{n} (l !! i).
+  Proof.
+    rewrite {1}/validN /list_validN Forall_lookup; split.
+    - intros Hl i. by destruct (l !! i) as [x|] eqn:?; [apply (Hl i)|].
+    - intros Hl i x Hi. move: (Hl i); by rewrite Hi.
+  Qed.
+  Lemma list_lookup_op l1 l2 i : (l1 ⋅ l2) !! i = l1 !! i ⋅ l2 !! i.
+  Proof.
+    revert i l2. induction l1 as [|x l1]; intros [|i] [|y l2];
+      by rewrite /= ?left_id_L ?right_id_L.
+  Qed.
+  Lemma list_lookup_core l i : core l !! i = core (l !! i).
+  Proof. revert i; induction l; intros [|i]; simpl; auto. Qed.
+
+  Lemma list_lookup_included l1 l2 : l1 ≼ l2 ↔ ∀ i, l1 !! i ≼ l2 !! i.
+  Proof.
+    split.
+    { intros [l Hl] i. exists (l !! i). by rewrite Hl list_lookup_op. }
+    revert l1. induction l2 as [|y l2 IH]=>-[|x l1] Hl.
+    - by exists [].
+    - destruct (Hl 0) as [[z|] Hz]; inversion Hz.
+    - by exists (y :: l2).
+    - destruct (IH l1) as [l3 ?]; first (intros i; apply (Hl (S i))).
+      destruct (Hl 0) as [[z|] Hz]; inversion_clear Hz; simplify_eq/=.
+      + exists (z :: l3); by constructor.
+      + exists (core x :: l3); constructor; by rewrite ?cmra_core_r.
+  Qed.
+
+  Definition list_cmra_mixin : CMRAMixin (list A).
+  Proof.
+    split.
+    - intros n l l1 l2; rewrite !list_dist_lookup=> Hl i.
+      by rewrite !list_lookup_op Hl.
+    - apply _.
+    - intros n l1 l2; rewrite !list_dist_lookup !list_lookup_validN=> Hl ? i.
+      by rewrite -Hl.
+    - intros l. rewrite list_lookup_valid. setoid_rewrite list_lookup_validN.
+      setoid_rewrite cmra_valid_validN. naive_solver.
+    - intros n x. rewrite !list_lookup_validN. auto using cmra_validN_S.
+    - intros l1 l2 l3; rewrite list_equiv_lookup=> i.
+      by rewrite !list_lookup_op assoc.
+    - intros l1 l2; rewrite list_equiv_lookup=> i.
+      by rewrite !list_lookup_op comm.
+    - intros l; rewrite list_equiv_lookup=> i.
+      by rewrite list_lookup_op list_lookup_core cmra_core_l.
+    - intros l; rewrite list_equiv_lookup=> i.
+      by rewrite !list_lookup_core cmra_core_idemp.
+    - intros l1 l2; rewrite !list_lookup_included=> Hl i.
+      rewrite !list_lookup_core. by apply cmra_core_preserving.
+    - intros n l1 l2. rewrite !list_lookup_validN.
+      setoid_rewrite list_lookup_op. eauto using cmra_validN_op_l.
+    - intros n l. induction l as [|x l IH]=> -[|y1 l1] [|y2 l2] Hl Hl';
+        try (by exfalso; inversion_clear Hl').
+      + by exists ([], []).
+      + by exists ([], x :: l).
+      + by exists (x :: l, []).
+      + destruct (IH l1 l2) as ([l1' l2']&?&?&?),
+          (cmra_extend n x y1 y2) as ([y1' y2']&?&?&?);
+          [inversion_clear Hl; inversion_clear Hl'; auto ..|]; simplify_eq/=.
+        exists (y1' :: l1', y2' :: l2'); repeat constructor; auto.
+  Qed.
+  Canonical Structure listR : cmraT := CMRAT list_cofe_mixin list_cmra_mixin.
+
+  Global Instance empty_list : Empty (list A) := [].
+  Global Instance list_cmra_unit : CMRAUnit listR.
+  Proof.
+    split.
+    - constructor.
+    - by intros l.
+    - by inversion_clear 1.
+  Qed.
+
+  Global Instance list_cmra_discrete : CMRADiscrete A → CMRADiscrete listR.
+  Proof.
+    split; [apply _|]=> l; rewrite list_lookup_valid list_lookup_validN=> Hl i.
+    by apply cmra_discrete_valid.
+  Qed.
+
+  Global Instance list_persistent l : (∀ x : A, Persistent x) → Persistent l.
+  Proof.
+    intros ?; apply list_equiv_lookup=> i.
+    by rewrite list_lookup_core (persistent (l !! i)).
+  Qed.
+
+  (** Internalized properties *)
+  Lemma list_equivI {M} l1 l2 : (l1 ≡ l2) ⊣⊢ (∀ i, l1 !! i ≡ l2 !! i : uPred M).
+  Proof. uPred.unseal; constructor=> n x ?. apply list_dist_lookup. Qed.
+  Lemma list_validI {M} l : (✓ l) ⊣⊢ (∀ i, ✓ (l !! i) : uPred M).
+  Proof. uPred.unseal; constructor=> n x ?. apply list_lookup_validN. Qed.
+End cmra.
+
+Arguments listR : clear implicits.
+
+Global Instance list_singletonM `{Empty A} : SingletonM nat A (list A) := λ n x,
+  replicate n ∅ ++ [x].
+
+Section properties.
+  Context {A : cmraT}.
+  Implicit Types l : list A.
+  Local Arguments op _ _ !_ !_ / : simpl nomatch.
+  Local Arguments cmra_op _ !_ !_ / : simpl nomatch.
+
+  Lemma list_op_app l1 l2 l3 :
+    length l2 ≤ length l1 → (l1 ++ l3) ⋅ l2 = (l1 ⋅ l2) ++ l3.
+  Proof.
+    revert l2 l3.
+    induction l1 as [|x1 l1]=> -[|x2 l2] [|x3 l3] ?; f_equal/=; auto with lia.
+  Qed.
+
+  Lemma list_lookup_validN_Some n l i x : ✓{n} l → l !! i ≡{n}≡ Some x → ✓{n} x.
+  Proof. move=> /list_lookup_validN /(_ i)=> Hl Hi; move: Hl. by rewrite Hi. Qed.
+  Lemma list_lookup_valid_Some l i x : ✓ l → l !! i ≡ Some x → ✓ x.
+  Proof. move=> /list_lookup_valid /(_ i)=> Hl Hi; move: Hl. by rewrite Hi. Qed.
+
+  Lemma list_op_length l1 l2 : length (l1 ⋅ l2) = max (length l1) (length l2).
+  Proof. revert l2. induction l1; intros [|??]; f_equal/=; auto. Qed.
+
+  Lemma replicate_valid n (x : A) : ✓ x → ✓ replicate n x.
+  Proof. apply Forall_replicate. Qed.
+
+  (* Singleton lists *)
+  Section singleton.
+    Context `{CMRAUnit A}.
+
+    Global Instance list_singletonM_ne n i :
+      Proper (dist n ==> dist n) (list_singletonM i).
+    Proof. intros l1 l2 ?. apply Forall2_app; by repeat constructor. Qed.
+    Global Instance list_singletonM_proper i :
+      Proper ((≡) ==> (≡)) (list_singletonM i) := ne_proper _.
+
+    Lemma elem_of_list_singletonM i z x : z ∈ {[i := x]} → z = ∅ ∨ z = x.
+    Proof.
+      rewrite elem_of_app elem_of_list_singleton elem_of_replicate. naive_solver.
+    Qed.
+    Lemma list_lookup_singletonM i x : {[ i := x ]} !! i = Some x.
+    Proof. induction i; by f_equal/=. Qed.
+    Lemma list_lookup_singletonM_ne i j x :
+      i ≠ j → {[ i := x ]} !! j = None ∨ {[ i := x ]} !! j = Some ∅.
+    Proof. revert j; induction i; intros [|j]; naive_solver auto with omega. Qed.
+    Lemma list_singletonM_validN n i x : ✓{n} {[ i := x ]} ↔ ✓{n} x.
+    Proof.
+      rewrite list_lookup_validN. split.
+      { move=> /(_ i). by rewrite list_lookup_singletonM. }
+      intros Hx j; destruct (decide (i = j)); subst.
+      - by rewrite list_lookup_singletonM.
+      - destruct (list_lookup_singletonM_ne i j x) as [Hi|Hi]; first done;
+          rewrite Hi; by try apply (cmra_unit_validN (A:=A)).
+    Qed.
+    Lemma list_singleton_valid  i x : ✓ {[ i := x ]} ↔ ✓ x.
+    Proof.
+      rewrite !cmra_valid_validN. by setoid_rewrite list_singletonM_validN.
+    Qed.
+    Lemma list_singletonM_length i x : length {[ i := x ]} = S i.
+    Proof.
+      rewrite /singletonM /list_singletonM app_length replicate_length /=; lia.
+    Qed.
+
+    Lemma list_core_singletonM i (x : A) : core {[ i := x ]} ≡ {[ i := core x ]}.
+    Proof.
+      rewrite /singletonM /list_singletonM /=.
+      induction i; constructor; auto using cmra_core_unit.
+    Qed.
+    Lemma list_op_singletonM i (x y : A) :
+      {[ i := x ]} ⋅ {[ i := y ]} ≡ {[ i := x ⋅ y ]}.
+    Proof.
+      rewrite /singletonM /list_singletonM /=.
+      induction i; constructor; rewrite ?left_id; auto.
+    Qed.
+    Lemma list_alter_singletonM f i x : alter f i {[i := x]} = {[i := f x]}.
+    Proof.
+      rewrite /singletonM /list_singletonM /=.
+      induction i; f_equal/=; auto.
+    Qed.
+    Global Instance list_singleton_persistent i (x : A) :
+      Persistent x → Persistent {[ i := x ]}.
+    Proof. intros. by rewrite /Persistent list_core_singletonM persistent. Qed.
+  End singleton.
+
+  (* Update *)
+  Lemma list_update_updateP (P : A → Prop) (Q : list A → Prop) l1 x l2 :
+    x ~~>: P → (∀ y, P y → Q (l1 ++ y :: l2)) → l1 ++ x :: l2 ~~>: Q.
+  Proof.
+    intros Hx%option_updateP' HP n mf; rewrite list_lookup_validN=> Hm.
+    destruct (Hx n (mf !! length l1)) as ([y|]&H1&H2); simpl in *; try done.
+    { move: (Hm (length l1)). by rewrite list_lookup_op list_lookup_middle. }
+    exists (l1 ++ y :: l2); split; auto.
+    apply list_lookup_validN=> i.
+    destruct (lt_eq_lt_dec i (length l1)) as [[?|?]|?]; subst.
+    - move: (Hm i); by rewrite !list_lookup_op !lookup_app_l.
+    - by rewrite list_lookup_op list_lookup_middle.
+    - move: (Hm i). rewrite !(cons_middle _ l1 l2) !assoc.
+      rewrite !list_lookup_op !lookup_app_r !app_length //=; lia.
+  Qed.
+
+  Lemma list_update_update l1 l2 x y : x ~~> y → l1 ++ x :: l2 ~~> l1 ++ y :: l2.
+  Proof.
+    rewrite !cmra_update_updateP => H; eauto using list_update_updateP with subst.
+  Qed.
+
+  (* Applying a local update at a position we own is a local update. *)
+  Global Instance list_alter_update `{LocalUpdate A Lv L} i :
+    LocalUpdate (λ L, ∃ x, L !! i = Some x ∧ Lv x) (alter L i).
+  Proof.
+    split; [apply _|]; intros n l1 l2 (x&Hi1&?) Hm; apply list_dist_lookup=> j.
+    destruct (decide (j = i)); subst; last first.
+    { by rewrite list_lookup_op !list_lookup_alter_ne // list_lookup_op. }
+    rewrite list_lookup_op !list_lookup_alter list_lookup_op Hi1.
+    destruct (l2 !! i) as [y|] eqn:Hi2; rewrite Hi2; constructor; auto.
+    eapply (local_updateN L), (list_lookup_validN_Some _ _ i); eauto.
+    by rewrite list_lookup_op Hi1 Hi2.
+  Qed.
+End properties.
+
+(** Functor *)
+Instance list_fmap_cmra_monotone {A B : cmraT} (f : A → B)
+  `{!CMRAMonotone f} : CMRAMonotone (fmap f : list A → list B).
+Proof.
+  split; try apply _.
+  - intros n l. rewrite !list_lookup_validN=> Hl i. rewrite list_lookup_fmap.
+    by apply (validN_preserving (fmap f : option A → option B)).
+  - intros l1 l2. rewrite !list_lookup_included=> Hl i. rewrite !list_lookup_fmap.
+    by apply (included_preserving (fmap f : option A → option B)).
+Qed.
+
+Program Definition listRF (F : rFunctor) : rFunctor := {|
+  rFunctor_car A B := listR (rFunctor_car F A B);
+  rFunctor_map A1 A2 B1 B2 fg := listC_map (rFunctor_map F fg)
+|}.
+Next Obligation.
+  by intros F ???? n f g Hfg; apply listC_map_ne, rFunctor_ne.
+Qed.
+Next Obligation.
+  intros F A B x. rewrite /= -{2}(list_fmap_id x).
+  apply list_fmap_setoid_ext=>y. apply rFunctor_id.
+Qed.
+Next Obligation.
+  intros F A1 A2 A3 B1 B2 B3 f g f' g' x. rewrite /= -list_fmap_compose.
+  apply list_fmap_setoid_ext=>y; apply rFunctor_compose.
+Qed.
+
+Instance listRF_contractive F :
+  rFunctorContractive F → rFunctorContractive (listRF F).
+Proof.
+  by intros ? A1 A2 B1 B2 n f g Hfg; apply listC_map_ne, rFunctor_contractive.
+Qed.
